rename 'freeFrom' -> 'isFreeFrom'

LinearMemory.v
@@ -19,20 +19,20 @@ Definition empty : Mem := fun _ => 0.
 Definition free : adr -> Mem -> Mem :=
   fun r m => set r 0 m.
     
-Definition freeFrom : adr -> Mem -> Prop :=
+Definition isFreeFrom : adr -> Mem -> Prop :=
   fun r m => forall r', r <= r' -> m r' = 0.
 
-Lemma freeFrom_free : forall (r : adr) (m : Mem) (n : nat), freeFrom r m -> free r (set r n m) = m.
+Lemma isFreeFrom_free : forall (r : adr) (m : Mem) (n : nat), isFreeFrom r m -> free r (set r n m) = m.
 Proof.
-  intros. unfold free, freeFrom, set in *. apply functional_extensionality. intros.
+  intros. unfold free, isFreeFrom, set in *. apply functional_extensionality. intros.
   remember (beq_nat x r) as b. destruct b.
   - symmetry in Heqb. apply beq_nat_true in Heqb. subst. erewrite H;auto.
   - reflexivity.
 Qed. 
 
-Lemma freeFrom_set : forall (r : adr) (m : Mem) (n : nat), freeFrom r m  ->  freeFrom (next r) (set r n m).
+Lemma isFreeFrom_set : forall (r : adr) (m : Mem) (n : nat), isFreeFrom r m  ->  isFreeFrom (next r) (set r n m).
 Proof.
-  unfold freeFrom, set, next. intros.  remember (beq_nat r' r) as b. destruct b;symmetry in Heqb.
+  unfold isFreeFrom, set, next. intros.  remember (beq_nat r' r) as b. destruct b;symmetry in Heqb.
   - apply beq_nat_true in Heqb. omega.
   - apply beq_nat_false in Heqb. apply H. omega.
 Qed. 
@@ -42,9 +42,9 @@ Proof.
   intros. unfold get, set. rewrite <- beq_nat_refl. reflexivity.
 Qed.
 
-Lemma freeFrom_first : freeFrom first empty.
+Lemma isFreeFrom_first : isFreeFrom first empty.
 Proof.
-  unfold freeFrom, first, empty. auto.
+  unfold isFreeFrom, first, empty. auto.
 Qed.
 End LinearMemory.
 
