Memory.v
@@ -13,15 +13,15 @@ Parameter empty : Mem.
 Parameter get : adr -> Mem -> nat.
 Parameter set : adr -> nat -> Mem -> Mem.
 Parameter free : adr -> Mem -> Mem.
-Parameter freeFrom : adr -> Mem -> Prop.
+Parameter isFreeFrom : adr -> Mem -> Prop.
 
-Axiom freeFrom_free : forall (r : adr) (m : Mem) (n : nat), freeFrom r m -> free r (set r n m) = m.
+Axiom isFreeFrom_free : forall (r : adr) (m : Mem) (n : nat), isFreeFrom r m -> free r (set r n m) = m.
 
-Axiom freeFrom_set : forall (r : adr) (m : Mem) (n : nat), freeFrom r m  ->  freeFrom (next r) (set r n m).
+Axiom isFreeFrom_set : forall (r : adr) (m : Mem) (n : nat), isFreeFrom r m  ->  isFreeFrom (next r) (set r n m).
 
 Axiom get_set : forall (r : adr) (m : Mem) (n : nat), get r (set r n m) = n.
 
-Axiom freeFrom_first : freeFrom first empty.
+Axiom isFreeFrom_first : isFreeFrom first empty.
 
 
 End Memory.
